Hoare/EstimateCalls.thy
@@ -1,0 +1,167 @@
+theory EstimateCalls
+
+imports TrTermination
+
+begin
+
+lemma call_gas_compare2 :
+"vctx_memory_usage v1 \<ge> 0 \<Longrightarrow>
+ at_least_eip150 net \<Longrightarrow>
+ vctx_stack v1 = x21 # x21a # x21b # x21c # x21d # x21e # x21f # x22f \<Longrightarrow>
+ Ccallgas x21 x21a x21b (\<not> vctx_account_existence v1 (vctx_recipient v1 c))
+                (vctx_gas v1) net
+                (calc_memu_extra (vctx_memory_usage v1) x21 x21a x21b x21c x21d x21e
+                  x21f) + 699
+       < meter_gas (Misc CALL) v1 c net"
+by (simp add:gas_simps  Ccallgas_def meter_gas_def C_def
+  thirdComponentOfC_def Gcallstipend_def vctx_stack_default_def
+  uint_nat cmem_new_helper  cmem_new_helper2
+calc_memu_extra_def min_L_helper min_L_helper2)
+
+lemma aux2 :
+ "x + z < y \<Longrightarrow> x \<ge> 0 \<Longrightarrow> uint (word_of_int x :: w256) + z < y"
+using word_convert_compare [of x]
+by auto
+
+lemma call_system_gas2 :
+"at_least_eip150 net \<Longrightarrow>
+ instruction_sem v1 c (Misc CALL) net =
+ InstructionToEnvironment (ContractCall args) v2 x33 \<Longrightarrow>
+  vctx_next_instruction v1 c = Some (Misc CALL) \<Longrightarrow>
+ vctx_memory_usage v1 \<ge> 0 \<Longrightarrow>
+ vctx_gas v1 > vctx_gas v2 + uint (callarg_gas args) + 699"
+apply (auto simp:instruction_sem_simps Let_def split:split_inst)
+apply (rule aux2)
+apply (rule call_gas_compare2, auto)
+apply (simp add:vctx_recipient_def vctx_next_instruction_default_def
+  vctx_stack_default_def)
+using callgas_ge0 memu_extra_ge0 apply force
+done
+
+lemma callcode_gas_compare2 :
+"at_least_eip150 net \<Longrightarrow>
+ vctx_memory_usage v1 \<ge> 0 \<Longrightarrow>
+ vctx_stack v1 = x21 # x21a # x21b # x21c # x21d # x21e # x21f # x22f \<Longrightarrow>
+ Ccallgas x21 x21a x21b (\<not> vctx_account_existence v1 (vctx_recipient v1 c))
+    (vctx_gas v1) net
+    (calc_memu_extra (vctx_memory_usage v1) x21 x21a x21b x21c x21d x21e x21f)
+    + 699   < meter_gas (Misc CALLCODE) v1 c net"
+by (simp add:gas_simps  Ccallgas_def meter_gas_def C_def
+  thirdComponentOfC_def Gcallstipend_def vctx_stack_default_def
+  uint_nat cmem_new_helper  cmem_new_helper2
+calc_memu_extra_def min_L_helper min_L_helper2 memu_code)
+
+lemma callcode_system_gas2 :
+"at_least_eip150 net \<Longrightarrow>
+ instruction_sem v1 c (Misc CALLCODE) net =
+ InstructionToEnvironment (ContractCall args) v2 x33 \<Longrightarrow>
+ vctx_next_instruction v1 c = Some (Misc CALLCODE) \<Longrightarrow>
+ vctx_memory_usage v1 \<ge> 0 \<Longrightarrow>
+ vctx_gas v1 > vctx_gas v2 + uint (callarg_gas args) + 699"
+apply (auto simp:instruction_sem_simps Let_def split:split_inst)
+apply (rule aux2)
+apply (rule callcode_gas_compare2, auto)
+apply (simp add:vctx_recipient_def vctx_next_instruction_default_def
+  vctx_stack_default_def)
+using callgas_ge0 memu_extra_ge0 apply force
+done
+
+lemma call_success_tight :
+  "at_least_eip150 net \<Longrightarrow>
+   g_vmstate st1 = InstructionContinue v1 \<Longrightarrow>
+   g_vmstate st2 = InstructionToEnvironment (ContractCall args) v2 hint \<Longrightarrow>
+   Continue st2 = next0 net (Continue st1) \<Longrightarrow>
+   Some (Misc CALL) = vctx_next_instruction v1 (g_cctx st1) \<Longrightarrow>
+   vctx_memory_usage v1 \<ge> 0 \<Longrightarrow>
+   system_gas st1 > system_gas st2 + 699"
+apply (auto simp add:next0_def next_state_def Let_def
+  system_gas_def vm_gas_def call_system_gas2
+  split:if_split_asm option.split_asm list.split_asm
+   contract_action.split_asm stack_hint.split_asm)
+using call_system_gas2 by force
+
+lemma callcode_success_tight :
+  "at_least_eip150 net \<Longrightarrow>
+   g_vmstate st1 = InstructionContinue v1 \<Longrightarrow>
+   g_vmstate st2 = InstructionToEnvironment (ContractCall args) v2 hint \<Longrightarrow>
+   Continue st2 = next0 net (Continue st1) \<Longrightarrow>
+   Some (Misc CALLCODE) = vctx_next_instruction v1 (g_cctx st1) \<Longrightarrow>
+   vctx_memory_usage v1 \<ge> 0 \<Longrightarrow>
+   system_gas st1 > system_gas st2 + 699"
+apply (auto simp add:next0_def next_state_def Let_def
+  system_gas_def vm_gas_def callcode_system_gas
+  split:if_split_asm option.split_asm list.split_asm
+   contract_action.split_asm stack_hint.split_asm)
+using callcode_system_gas2 by force
+
+lemma call_tight :
+  "at_least_eip150 net \<Longrightarrow>
+   g_vmstate st1 = InstructionContinue v1 \<Longrightarrow>
+   g_vmstate st2 = InstructionToEnvironment (ContractCall args) v2 hint \<Longrightarrow>
+   Continue st2 = next0 net (Continue st1) \<Longrightarrow>
+   vctx_memory_usage v1 \<ge> 0 \<Longrightarrow>
+   system_gas st1 > system_gas st2 + 699"
+using call_success_tight callcode_success_tight call_success2
+by metis
+
+fun count_call :: "global_state \<Rightarrow> int" where
+"count_call (Continue g) = (case g_vmstate g of
+   InstructionToEnvironment (ContractCall _) v hint \<Rightarrow> 1
+ | _ \<Rightarrow> 0)"
+| "count_call _ = 0"
+
+(*
+
+fun iter_next :: "network \<Rightarrow> global_state \<Rightarrow> nat \<Rightarrow> global_state" where
+"iter_next net g 0 = g"
+| "iter_next net g (Suc n) = iter_next net (next0 net g) n"
+
+fun count_calls :: "network \<Rightarrow> global_state \<Rightarrow> nat \<Rightarrow> int" where
+"count_calls net g n = (\<Sum>i=1..n. count_call (iter_next net g i))"
+
+lemma iter_next_next :
+  "iter_next net (next0 net st) i = iter_next net st (Suc i)"
+by auto
+
+declare iter_next.simps [simp del]
+declare count_calls.simps [simp del]
+
+lemma count_calls_next :
+  "count_calls net (next0 net st) num +
+   count_call (next0 net st) =
+   count_calls net st (num+1)"
+apply auto
+apply (subst count_calls.simps)
+apply (subst count_calls.simps)
+apply (subst iter_next_next)
+
+lemma estimate_calls_continue :
+"      at_least_eip150 net \<Longrightarrow>
+       iter_next net (Continue st) num = Continue st2 \<Longrightarrow>
+       count_calls net (Continue st) num * 699
+           \<le> system_gas st - system_gas st2 \<Longrightarrow>
+       at_least_eip150 net \<Longrightarrow>
+       Continue st = next0 net (Continue st1) \<Longrightarrow>
+       iter_next net (Continue st1) (Suc num) = Continue st2 \<Longrightarrow>
+       g_vmstate st2 = InstructionContinue x1 \<Longrightarrow>
+       count_calls net (Continue st1) (Suc num) * 699
+       \<le> system_gas st1 - system_gas st2"
+apply auto
+
+lemma estimate_calls :
+  "at_least_eip150 net \<Longrightarrow>
+   iter_next net (Continue st1) num = Continue st2 \<Longrightarrow>
+   count_calls net (Continue st1) num * 699 \<le>
+   system_gas st1 - system_gas st2"
+apply (induction num arbitrary:st1 st2, simp)
+apply (case_tac "g_vmstate st2",auto)
+
+*)
+
+(*
+"count_calls net g 0 = 0"
+| "count_calls net g (Suc n) =
+     count_call g + count_calls net (next0 net g) n"
+*)
+
+end
